eval_mkApps_tFix_inv

erasure/theories/EEtaExpanded.v
@@ -57,8 +57,8 @@ Variable Σ : global_declarations.
 Local Unset Elimination Schemes.
  
 Inductive expanded (Γ : list nat): term -> Prop :=
-| expanded_tRel (n : nat) : nth n Γ 0 = 0 -> expanded Γ (tRel n)
-| expanded_tRel_app (n : nat) args : nth n Γ 0 <= #|args| -> Forall (expanded Γ) args -> expanded Γ (mkApps (tRel n) args)
+| expanded_tRel (n : nat) : nth_error Γ n = Some 0 -> expanded Γ (tRel n)
+| expanded_tRel_app (n : nat) args m : nth_error Γ n = Some m -> forall Hle : m <= #|args|, Forall (expanded Γ) args -> expanded Γ (mkApps (tRel n) args)
 | expanded_tLambda (na : name) (body : term) : (* expanded Γ ty -> *) expanded (0 :: Γ) body -> expanded Γ (tLambda na body)
 | expanded_tLetIn (na : name) (def : term) (body : term) : expanded Γ def (* -> expanded Γ def_ty *) -> expanded (0 :: Γ) body -> expanded Γ (tLetIn na def body)
 | expanded_mkApps (f : term) (args : list term) : negb (isConstruct f || isFix f || isRel f) -> expanded Γ f -> Forall (expanded Γ) args -> expanded Γ (mkApps f args)
@@ -91,10 +91,11 @@ End expanded.
 
 Lemma expanded_ind :
   ∀ (Σ : global_declarations) (P : list nat → term → Prop),
-    (∀ (Γ : list nat) (n : nat), nth n Γ 0 = 0 → P Γ (tRel n))
-    → (∀ (Γ : list nat) (n : nat) (args : list term),
-	        nth n Γ 0 ≤ #|args|
-        → Forall (expanded Σ Γ) args
+    (∀ (Γ : list nat) (n : nat), nth_error Γ n = Some 0 → P Γ (tRel n))
+    → (∀ (Γ : list nat) (n : nat) (args : list term) (m : nat),
+         nth_error Γ n = Some m ->
+          (m ≤ #|args|) ->
+	        Forall (expanded Σ Γ) args
         → Forall (P Γ) args 
         → P Γ (mkApps (tRel n) args))
     → (∀ (Γ : list nat) (na : name) (body : term),
@@ -187,6 +188,23 @@ From MetaCoq.SafeChecker Require Import PCUICWfEnv.
      
 From MetaCoq.Erasure Require Import EAst EAstUtils EInduction EArities Extract Prelim
     ELiftSubst ESpineView ECSubst.
+
+Hint Rewrite repeat_length : len.
+
+Lemma expanded_closed Σ Γ t : 
+  expanded Σ Γ t -> ELiftSubst.closedn #|Γ| t.
+Proof.
+  induction 1; cbn; eauto.
+  all: try now (rewrite ?closedn_mkApps; rtoProp; repeat solve_all).
+  - eapply nth_error_Some_length in H. now eapply Nat.ltb_lt.
+  - rewrite closedn_mkApps. rtoProp. split. cbn.
+    + eapply nth_error_Some_length in H. now eapply Nat.ltb_lt.
+    + solve_all.
+  - rtoProp. repeat split. eauto. solve_all. revert b. now len.
+  - rewrite closedn_mkApps. rtoProp. repeat split; cbn; solve_all.
+    revert  b. now len.
+  - solve_all. revert b. now len.
+Qed.
 
 Local Open Scope string_scope.
 Set Asymmetric Patterns.
@@ -326,14 +344,14 @@ Section isEtaExp.
   Equations? isEtaExp (Γ : list nat) (e : EAst.term) : bool
     by wf e (fun x y : EAst.term => size x < size y) :=
     isEtaExp Γ e with TermSpineView.view e := {
-    | tRel i => Nat.eqb (nth i Γ 0) 0
+    | tRel i => option_default (Nat.eqb 0) (nth_error Γ i) false
     | tEvar ev args => forallb_InP args (fun x H => isEtaExp Γ x)
     | tLambda na M => isEtaExp (0 :: Γ) M
     | tApp u v napp nnil with expanded_head_viewc u := 
       { | expanded_head_construct ind i => isEtaExp_app ind i (List.length v) && forallb_InP v (fun x H => isEtaExp Γ x)
         | expanded_head_fix mfix idx => isEtaExp_fixapp mfix idx (List.length v) && 
                                         forallb_InP mfix (fun x H => isEtaExp (rev_map (S ∘ rarg) mfix ++ Γ) x.(dbody)) && forallb_InP v (fun x H => isEtaExp Γ x)
-        | expanded_head_rel n => (nth n Γ 0 <=? List.length v) && forallb_InP v (fun x H => isEtaExp Γ x) 
+        | expanded_head_rel n => option_default (fun m => m <=? List.length v) (nth_error Γ n) false && forallb_InP v (fun x H => isEtaExp Γ x) 
         | expanded_head_other _ _ => isEtaExp Γ u && forallb_InP v (fun x H => isEtaExp Γ x) }
     | tLetIn na b b' => isEtaExp Γ b && isEtaExp (0 :: Γ) b'
     | tCase ind c brs => isEtaExp Γ c && forallb_InP brs (fun x H => isEtaExp (repeat 0 #|x.1| ++ Γ) x.2)
@@ -383,7 +401,7 @@ Section isEtaExp.
     isEtaExp Γ (mkApps f v) = match expanded_head_viewc f with 
       | expanded_head_construct ind i => isEtaExp_app ind i #|v| && forallb (isEtaExp Γ) v
       | expanded_head_fix mfix idx => isEtaExp_fixapp mfix idx #|v| && forallb (fun x => isEtaExp (rev_map (S ∘ rarg) mfix ++ Γ) x.(dbody)) mfix && forallb (isEtaExp Γ) v
-      | expanded_head_rel n => (nth n Γ 0 <=? List.length v) && forallb (fun x => isEtaExp Γ x) v
+      | expanded_head_rel n => option_default (fun m => m <=? List.length v) (nth_error Γ n) false && forallb (fun x => isEtaExp Γ x) v
       | expanded_head_other t discr => isEtaExp Γ f && forallb (isEtaExp Γ) v
     end.
   Proof.
@@ -402,14 +420,16 @@ Section isEtaExp.
     isEtaExp Γ (mkApps f v) = match expanded_head_viewc f with 
       | expanded_head_construct ind i => isEtaExp_app ind i #|v| && forallb (isEtaExp Γ) v
       | expanded_head_fix mfix idx => isEtaExp_fixapp mfix idx #|v| && forallb (fun x => isEtaExp (rev_map (S ∘ rarg) mfix ++ Γ) x.(dbody)) mfix && forallb (isEtaExp Γ) v
-      | expanded_head_rel n => (nth n Γ 0 <=? List.length v) && forallb (fun x => isEtaExp Γ x) v
+      | expanded_head_rel n => option_default (fun m => m <=? List.length v) (nth_error Γ n) false && forallb (fun x => isEtaExp Γ x) v
       | expanded_head_other t discr => isEtaExp Γ f && forallb (isEtaExp Γ) v
     end.
   Proof.
     intros napp.
     destruct v using rev_case; simp_eta.
     - destruct expanded_head_viewc; rewrite ? andb_true_r //. cbn. unfold isEtaExp_fixapp. now destruct (nth_error); cbn.
-      cbn. destruct (Nat.eqb_spec (nth n Γ 0) 0), (Nat.leb_spec (nth n Γ 0) 0); try reflexivity; lia.
+      cbn.
+      destruct (nth_error Γ n) as [m | ]; cbn; try reflexivity.
+      destruct (Nat.eqb_spec 0 m), (Nat.leb_spec m 0); try reflexivity; lia.
     - rewrite isEtaExp_mkApps_nonnil //. destruct v; cbn; try congruence.      
   Qed.
 
@@ -435,7 +455,9 @@ Section isEtaExp.
         eapply isEtaExp_app_mon; tea; lia. 
         eapply All_app_inv; eauto.
       + cbn in *; congruence.
-      + simp_eta in et. eapply Nat.eqb_eq in et. rewrite et.
+      + simp_eta in et.
+       destruct (nth_error Γ n) as [m | ] eqn:Heq; cbn in et; try eauto.
+        eapply Nat.eqb_eq in et. rewrite <- et.
         rtoProp. split. cbn. eauto.
         solve_all. eapply All_app_inv; solve_all.
       + rewrite et forallb_app /=. rtoProp; repeat solve_all. 
@@ -455,6 +477,7 @@ Section isEtaExp.
         * solve_all. eapply All_app_inv; solve_all. eapply All_app_inv; solve_all.
       + rewrite -mkApps_app. rewrite isEtaExp_mkApps //.
         cbn [expanded_head_viewc]. rtoProp. split.
+        destruct (nth_error Γ n) as [m | ] eqn:Heq; cbn in H0; eauto.
         cbn. eapply Nat.leb_le in H0. eapply Nat.leb_le. revert H0. len. lia.
         solve_all. eapply All_app_inv. 2: eapply All_app_inv. all: solve_all.
       + rewrite -mkApps_app. rewrite isEtaExp_mkApps //.
@@ -472,11 +495,33 @@ Section isEtaExp.
   Proof.
   Admitted.
 
+  Lemma isEtaExp_closed Γ t : 
+    isEtaExp Γ t -> closedn #|Γ| t.
+  Proof.
+    funelim (isEtaExp Γ t); simp_eta; cbn [closedn];
+    rewrite ?closedn_mkApps; rtoProp; (try toAll); repeat solve_all.
+    - destruct nth_error eqn:Hn; cbn in H; try easy.
+      eapply nth_error_Some_length in Hn. now eapply Nat.ltb_lt.
+    - eapply a in b. 2: f_equal. revert b. now len.
+    - easy.
+    - eapply a in b. 2: f_equal. revert b. now len.
+    - cbn. solve_all. eapply a in b. 2: reflexivity. revert b. now len.
+    - destruct nth_error eqn:Hn; cbn in H1; try easy.
+      eapply nth_error_Some_length in Hn. now eapply Nat.ltb_lt.
+  Qed.
+
+  Lemma option_default_ext {A B} (f : A -> B) x1 x2 d :
+    x1 = x2 -> option_default f x1 d = option_default f x2 d.
+  Proof.
+    now intros ->.
+  Qed.
+
   Lemma etaExp_csubst' a k b n Γ Δ : 
     #|Γ| = k ->
-    closed a -> isEtaExp [] a -> isEtaExp (Γ ++ [n] ++ Δ) b -> isEtaExp (Γ ++ Δ) (ECSubst.csubst a k b).
+    isEtaExp [] a -> isEtaExp (Γ ++ [n] ++ Δ) b -> isEtaExp (Γ ++ Δ) (ECSubst.csubst a k b).
   Proof.
-    intros Hk Hcl. 
+    intros Hk H.
+    assert (Hcl : closed a) by now eapply isEtaExp_closed in H. revert H.
     remember (Γ ++ [n] ++ Δ)%list as Γ_.
     funelim (isEtaExp Γ_ b); try simp_eta; eauto; try fold csubst;
       try toAll; repeat solve_all; subst.
@@ -485,14 +530,11 @@ Section isEtaExp.
         rewrite <- (app_nil_r (Γ0 ++ Δ)).
         eapply expanded_lift with(Γ' := []); eassumption. 
         eassumption.
-      + rewrite app_nth2. lia.
-        rewrite app_nth2 in H0. lia.
-        eapply Nat.eqb_eq in H0. eapply Nat.eqb_eq.
-        rewrite <- H0 at 2. destruct i. lia.
-        cbn [Nat.pred].
-        rewrite app_nth2. cbn. lia. f_equal. cbn. lia.
-      + rewrite !app_nth1 in H0 |- *; try lia.
-        eapply Nat.eqb_eq in H0. eapply Nat.eqb_eq. lia.
+      + rewrite nth_error_app2. lia.
+        rewrite !nth_error_app2 in H0. lia. cbn. lia.
+        erewrite option_default_ext; eauto.
+        f_equal. destruct i; cbn; lia.
+      + now rewrite !nth_error_app1 in H0 |- *; try lia.
     - eapply H with (Γ := 0 :: Γ0); cbn; eauto.
     - move/andP: H2 => [] etab etab'. simp_eta.
       apply/andP. split; eauto.
@@ -525,13 +567,11 @@ Section isEtaExp.
         eassumption.
       + rewrite isEtaExp_mkApps; eauto. cbn [expanded_head_viewc].
         rtoProp. split. 2: solve_all.
-        eapply Nat.leb_le in H1. eapply Nat.leb_le. rewrite app_nth2 in H1 |- *; try lia.
-        len. rewrite <- H1. rewrite !app_nth2; cbn; try lia.
-        eapply Nat.eq_le_incl. f_equal. lia.
+        rewrite !nth_error_app2 in H1 |- *; cbn; try lia.
+        len. erewrite option_default_ext; eauto. f_equal.
+        destruct n; cbn; lia.
       + rewrite isEtaExp_mkApps; eauto. cbn [expanded_head_viewc].
-        rtoProp. split. 2: solve_all. rewrite app_nth1 in H1 |- *; try lia.
-        eapply Nat.leb_le in H1. eapply Nat.leb_le. 
-        len. rewrite <- H1. rewrite !app_nth1; cbn; try lia.
+        rtoProp. split. 2: solve_all. len. now rewrite !nth_error_app1 in H1 |- *; try lia.
     - rewrite csubst_mkApps /=.
       move/andP: H2 => [] eu ev.
       eapply isEtaExp_mkApps_intro => //. 2: solve_all.
@@ -539,7 +579,7 @@ Section isEtaExp.
   Qed.
 
   Lemma etaExp_csubst a b n : 
-    closed a -> isEtaExp []a -> isEtaExp [n] b -> isEtaExp [] (ECSubst.csubst a 0 b).
+    isEtaExp []a -> isEtaExp [n] b -> isEtaExp [] (ECSubst.csubst a 0 b).
   Proof.
     intros.
     eapply etaExp_csubst' with (Γ := []); eauto.
@@ -557,15 +597,11 @@ Section isEtaExp.
     funelim (isEtaExp Γ_ b); try simp_eta; eauto; try fold csubst;
       try toAll; try now repeat solve_all; subst.
     - intros. simp isEtaExp ; cbn. destruct (Nat.compare_spec #|Γ0| i) => //; simp_eta.
-      + rewrite app_nth2 in H0; try lia. subst. rewrite minus_diag in H0. now cbn in H0.
-      + rewrite app_nth2. lia.
-        rewrite app_nth2 in H0. lia.
-        eapply Nat.eqb_eq in H0. eapply Nat.eqb_eq.
-        rewrite <- H0 at 2. destruct i. lia.
-        cbn [Nat.pred].
-        rewrite app_nth2. cbn. lia. f_equal. cbn. lia.
-      + rewrite !app_nth1 in H0 |- *; try lia.
-        eapply Nat.eqb_eq in H0. eapply Nat.eqb_eq. lia.
+      + rewrite nth_error_app2 in H0; try lia; cbn in H0; try easy. subst. rewrite minus_diag in H0. cbn in H0. easy.
+      + rewrite !nth_error_app2 in H0 |- *; cbn; try lia.
+        erewrite option_default_ext; eauto. f_equal.
+        destruct i; cbn; lia.
+      + now rewrite !nth_error_app1 in H0 |- *; try lia.
     - intros. solve_all. eapply a; eauto. solve_all.
     - eapply H with (Γ := 0 :: Γ0); cbn -[isEtaExp]; eauto. 
     - solve_all. move/andP: H2 => [] etab etab'. simp_eta.
@@ -606,7 +642,7 @@ Section isEtaExp.
       + rewrite isEtaExp_mkApps => //. cbn [expanded_head_viewc].
         rtoProp. repeat split; eauto.
         * unfold isEtaExp_fixapp. rewrite Hnth. len. destruct H2 as [Hn H2].
-          subst. rewrite app_nth2 in Hn; try lia.
+          subst. rewrite nth_error_app2 in Hn; try lia.
           rewrite minus_diag in Hn. cbn in Hn. eapply Nat.ltb_lt.
           eapply Nat.leb_le in Hn. lia.        
         * cbn in Hcl. solve_all. 
@@ -617,15 +653,16 @@ Section isEtaExp.
         * destruct H2. solve_all. eapply a ;eauto. solve_all.          
       + rewrite isEtaExp_mkApps; eauto. cbn [expanded_head_viewc].
         rtoProp. intros. destruct H2. split. 2:{ solve_all. eapply a; eauto. solve_all. }
-        eapply Nat.leb_le in H2. eapply Nat.leb_le. rewrite app_nth2 in H2 |- *; try lia.
-        len. rewrite <- H2. rewrite !app_nth2; cbn; try lia.
-        eapply Nat.eq_le_incl. destruct (n - #|Γ0|) eqn:E. lia. f_equal. lia.
+        rewrite !nth_error_app2 in H2 |- *; try lia.
+        rewrite (nth_error_app2 ([S (EAst.rarg d)])) in H2; cbn; try lia.
+        len.
+        erewrite option_default_ext. eauto. f_equal.
+        destruct n; cbn; lia.
       + rewrite isEtaExp_mkApps; eauto. cbn [expanded_head_viewc].
         intros. destruct H2.
         rtoProp. split. 2:{ solve_all. eapply a; eauto. solve_all. }
-        rewrite app_nth1 in H2 |- *; try lia.
-        eapply Nat.leb_le in H2. eapply Nat.leb_le. 
-        len. rewrite <- H2. rewrite !app_nth1; cbn; try lia.
+        len.
+        now rewrite !nth_error_app1 in H2 |- *; try lia.
     - intros. rtoProp. rewrite csubst_mkApps /=.
       eapply isEtaExp_mkApps_intro => //. 2:{ solve_all. eapply a; eauto. solve_all. }
       eapply H; eauto.
@@ -633,23 +670,24 @@ Section isEtaExp.
   
   Lemma isEtaExp_substl Γ Δ s t : 
     #|Γ| = #|s| ->
-    Forall (closedn 0) s ->
     forallb (isEtaExp []) s -> isEtaExp (Γ ++ Δ) t ->
     isEtaExp Δ (substl s t).
   Proof.
     induction s in Γ, t |- *; simpl; auto;
     rtoProp; intuition eauto using etaExp_csubst.
     - destruct Γ; eauto; cbn in *; lia.
-    - invs H0. destruct Γ; cbn in H; invs H.
+    - destruct Γ; cbn in H; invs H.
       eapply IHs; eauto. eapply etaExp_csubst' with (Γ := []); eauto.
   Qed.
 
-  Lemma isEtaExp_fixsubstl Δ mfix idx t : 
-    closed (EAst.tFix mfix idx) ->
+  Lemma isEtaExp_fixsubstl Δ mfix t : 
     forallb (fun x => isEtaExp (rev_map (S ∘ rarg) mfix) x.(dbody)) mfix ->
     isEtaExp ((rev_map (S ∘ rarg) mfix) ++ Δ) t ->
     isEtaExp Δ (substl (fix_subst mfix) t).
   Proof.
+    intros Hall Heta.
+    assert (Hcl : closed (EAst.tFix mfix 0) ). { cbn. solve_all. eapply isEtaExp_closed in H. revert H. now len. }
+    revert Hcl Hall Heta.  
     intros Hcl Hall Heta.
     cbn in Hcl. solve_all.
     unfold fix_subst.
@@ -687,7 +725,6 @@ Section isEtaExp.
     erewrite (isEtaExp_substl _ []); eauto.
     - shelve.
     - solve_all. eapply All_skipn. solve_all.
-    - rewrite forallb_rev forallb_skipn //.
     - rewrite app_nil_r. eauto.
     Unshelve. len. now rewrite List.skipn_length.  
   Qed.
@@ -721,39 +758,33 @@ Section isEtaExp.
   Qed. 
   
   Lemma isEtaExp_cunfold_fix mfix idx n f : 
-    forallb (closedn 0 ∘ dbody) mfix ->
     forallb (isEtaExp (rev_map (S ∘ rarg) mfix) ∘ dbody) mfix ->
     Ee.cunfold_fix mfix idx = Some (n, f) ->
     isEtaExp [] f.
   Proof.
-    intros hcl heta.
+    intros heta.
     unfold Ee.cunfold_fix.
     destruct nth_error eqn:heq => //.
     intros [= <- <-] => /=.
     eapply isEtaExp_fixsubstl.
-    - cbn. solve_all. unfold EAst.test_def. eapply closed_upwards; eauto. lia.
     - solve_all.
-    - solve_all. eapply All_nth_error in heta as []; eauto.
-      now rewrite app_nil_r.
-      Unshelve. eauto.
+    - rewrite app_nil_r. solve_all. eapply All_nth_error in heta; eauto.
   Qed.
   
   Lemma isEtaExp_cunfold_cofix mfix idx n f : 
-    forallb (closedn 0 ∘ dbody) mfix ->
     forallb (isEtaExp (repeat 0 #|mfix|) ∘ dbody) mfix ->
     Ee.cunfold_cofix mfix idx = Some (n, f) ->
     isEtaExp [] f.
   Proof.
-    intros hcl heta.
+    intros heta.
     unfold Ee.cunfold_cofix.
     destruct nth_error eqn:heq => //.
     intros [= <- <-] => /=.
     eapply isEtaExp_substl.
-    4:{ solve_all. eapply nth_error_all in heta; eauto. rewrite app_nil_r. eapply heta. }
+    3:{ solve_all. eapply nth_error_all in heta; eauto. rewrite app_nil_r. eapply heta. }
     - len. now rewrite cofix_subst_length.
-    - unfold cofix_subst. generalize #|mfix|. clear - hcl. induction n; econstructor; eauto.
-      cbn. solve_all. eapply closed_upwards; eauto. lia.
-    - eapply isEtaExp_cofix_subst in heta. solve_all.
+    - solve_all. unfold cofix_subst. generalize #|mfix|. clear - heta. induction n; econstructor; eauto.
+      simp_eta. solve_all. now rewrite app_nil_r.
   Qed.
 
   Lemma isEtaExp_tApp Γ f u : isEtaExp Γ (mkApps f u) -> 
@@ -761,7 +792,7 @@ Section isEtaExp.
     match expanded_head_viewc hd with
       | expanded_head_construct ind i => isEtaExp_app ind i #|v| && forallb (isEtaExp Γ) v
       | expanded_head_fix mfix idx => isEtaExp_fixapp mfix idx #|v| && forallb (fun x => isEtaExp (rev_map (S ∘ rarg) mfix ++ Γ) x.(dbody)) mfix && forallb (isEtaExp Γ) v
-      | expanded_head_rel n => (nth n Γ 0 <=? List.length v) && forallb (fun x => isEtaExp Γ x) v
+      | expanded_head_rel n => (option_default (fun m => m <=? List.length v) (nth_error Γ n) false) && forallb (fun x => isEtaExp Γ x) v
       | expanded_head_other t discr => isEtaExp Γ hd && forallb (isEtaExp Γ) v
       end. (* 
     | expanded_head_construct kn c => isEtaExp_app Σ kn c #|args| && forallb (isEtaExp Σ) args
@@ -851,7 +882,7 @@ Lemma isEtaExp_expanded Σ Γ t :
   isEtaExp Σ Γ t -> expanded Σ Γ t.
 Proof.
   funelim (isEtaExp Σ Γ t); intros; solve_all; eauto.
-  - econstructor. now eapply Nat.eqb_eq.
+  - econstructor. destruct (nth_error); invs H. f_equal. eapply Nat.eqb_eq in H1; eauto.
   - todo "tVar".
   - rewrite forallb_InP_spec in H0. eapply forallb_Forall in H0. eapply In_All in H.
     todo "tEvar".
@@ -873,7 +904,8 @@ Proof.
     eapply expanded_tFix.
     all: try now solve_all.
     eapply Nat.ltb_lt in H1. lia.
-  - rtoProp. econstructor. eapply Nat.leb_le; eauto.  rewrite forallb_InP_spec in H1.
+  - rtoProp. destruct (nth_error) eqn:Hn; invs H0.
+    econstructor. eauto. eapply Nat.leb_le; eauto.  rewrite forallb_InP_spec in H1.
     eapply Forall_forall. solve_all. eapply H; eauto.
     eapply All_Forall, Forall_forall in H1; eauto.
   - eapply andb_true_iff in H1 as []. rewrite forallb_InP_spec in H2. eapply forallb_Forall in H2.
@@ -891,9 +923,9 @@ Proof.
     (try (eapply andb_true_iff; split; eauto));
     (try eapply forallb_Forall); 
     eauto).
-  - eapply Nat.eqb_eq; eauto.
+  - rewrite H. eapply Nat.eqb_eq; eauto.
   - rewrite isEtaExp_mkApps //. cbn [expanded_head_viewc].
-    rtoProp. split. 2: solve_all. now eapply Nat.leb_le.
+    rtoProp. split. 2: solve_all. rewrite H.  now eapply Nat.leb_le.
   - eapply isEtaExp_mkApps_intro; eauto. solve_all. 
   - rewrite isEtaExp_mkApps //. cbn [expanded_head_viewc]. rtoProp. repeat split.
     + unfold isEtaExp_fixapp. rewrite H4. eapply Nat.ltb_lt. lia.
@@ -918,7 +950,6 @@ Fixpoint isEtaExp_env (Σ : global_declarations) :=
   | [] => true
   | decl :: Σ => isEtaExp_decl Σ decl.2 && isEtaExp_env Σ
   end.
-
 
 Lemma closedn_mkApps k f l : closedn k (mkApps f l) = closedn k f && forallb (closedn k) l.
 Proof.
@@ -997,7 +1028,7 @@ Lemma isEtaExp_tApp' {Σ} {Γ} {f u} : isEtaExp Σ Γ (tApp f u) ->
     isEtaExp_fixapp mfix idx #|args| && forallb (fun d => isEtaExp Σ (rev_map (fun  d => 1 + d.(rarg)) mfix ++ Γ) d.(dbody)) mfix && forallb (isEtaExp Σ Γ) args
   | expanded_head_rel n => 
     args <> [] /\ f = mkApps hd (remove_last args) /\ u = last args u /\ 
-    (nth n Γ 0 <=? List.length args) && forallb (fun x => isEtaExp Σ Γ x) args
+    option_default (fun m => m <=? List.length args) (nth_error Γ n) false && forallb (fun x => isEtaExp Σ Γ x) args
   | expanded_head_other _ discr => 
     [&& isEtaExp Σ Γ hd, forallb (isEtaExp Σ Γ) args, isEtaExp Σ Γ f & isEtaExp Σ Γ u]
   end.
@@ -1143,110 +1174,271 @@ Qed.
 
 Arguments lookup_inductive_pars_constructor_pars_args {Σ ind n pars args}.
 
+Lemma remove_last_length {X} {l : list X} : 
+  #|remove_last l| = match l with nil => 0 | _ => #|l| - 1 end.
+Proof.
+  unfold remove_last. rewrite firstn_length.
+  destruct l; cbn; lia.
+Qed.
+
+Lemma remove_last_length' {X} {l : list X} : 
+  l <> nil -> 
+  #|remove_last l| = #|l| - 1.
+Proof.
+  intros. rewrite remove_last_length. destruct l; try congruence; lia.
+Qed.
+ 
+Local Hint Rewrite @remove_last_length : len.
+
+Lemma eval_mkApps_tFix_inv {wfl : WcbvFlags} Σ mfix idx args v :
+with_guarded_fix ->
+  eval Σ (mkApps (tFix mfix idx) args) v ->
+ ((args = [] /\ v = tFix mfix idx) \/ exists args' n, args <> nil /\ ∥ All2 (eval Σ) (skipn n args) args'∥ /\ #|args| = n + #| args'| /\
+                                                                     v = mkApps (tFix mfix idx) (firstn n args ++ args')) \/
+ (exists n b, args <> nil /\ cunfold_fix mfix idx = Some (n, b) /\ n < #|args|).
+Proof.
+ revert v.
+ induction args using List.rev_ind; intros v wg ev.
+ + left. now depelim ev.
+ + rewrite mkApps_app in ev.
+   cbn in *.
+   depelim ev.
+   all: try (eapply IHargs in ev1 as [[(-> & Heq) | (args' & n & ? & ? & ? & Heq)] | (? & ? & ? & ? & ?)]; eauto; rewrite ?Heq; try solve_discr; try congruence;
+     len; rewrite ?Heq; rewrite Nat.add_comm; eauto 9).
+   * right. repeat eexists. destruct args; cbn; congruence. eauto. lia.
+   * right. repeat eexists. destruct args; cbn; congruence. eauto. lia.
+   * eapply IHargs in ev1 as [[(-> & Heq) | (args' & n & ? & ? & ? & Heq)] | (? & ? & ? & ? & ?)]; eauto; rewrite ?Heq; try solve_discr; try congruence.
+     -- invs H. cbn in *. right. repeat eexists. congruence. eauto. lia.
+     -- invs H2. right. repeat eexists. destruct args; cbn; congruence. eauto. len. rewrite firstn_length. lia.
+     -- right. repeat eexists.    destruct args; cbn; congruence. eauto. len. lia.
+   * eapply IHargs in ev1 as [[(-> & Heq) | (args' & n & ? & ? & ? & Heq)] | (? & ? & ? & ? & ?)]; eauto; rewrite ?Heq; try solve_discr; try congruence.
+     -- invs H. left. right. exists [av]. cbn. exists 0. repeat split. congruence. repeat econstructor. eauto.
+     -- invs H2. left. right. sq. exists (args' ++ [av])%list, n. repeat split. destruct args; cbn; congruence. 
+        2: len; rewrite H1; lia. rewrite skipn_app.
+        assert (n - #|args| = 0) as -> by lia. rewrite skipn_0.
+        eapply All2_app. eauto. repeat econstructor; eauto.
+        rewrite firstn_app. assert (n - #|args| = 0) as -> by lia.
+        cbn. rewrite app_nil_r.
+        now rewrite !mkApps_app.
+     -- right. repeat eexists. destruct args; cbn; congruence. eauto. len. lia.
+   * eapply IHargs in ev1 as [[(-> & Heq) | (args' & n & ? & ? & ? & Heq)] | (? & ? & ? & ? & ?)]; eauto; rewrite ?Heq; try solve_discr; try congruence; subst.
+     -- rewrite wg in i. cbn in i. easy.
+     -- rewrite wg in i. rewrite isFixApp_mkApps in i => //. cbn in i. destruct EAst.isLambda; easy.
+     -- right. repeat eexists. destruct args; cbn; congruence. eauto. len. lia.
+   * inv i.
+Qed.
+
+Lemma Forall_last {A} (P : A -> Prop) a l : l <> [] -> Forall P l -> P (last l a).
+Proof.
+  intros. induction H0.
+  - congruence.
+  - destruct l.
+    + cbn. eauto.
+    + cbn. eapply IHForall. congruence.
+Qed.
+
 Lemma eval_etaexp {fl : Ee.WcbvFlags} {Σ a a'} : 
   isEtaExp_env Σ ->
   wf_glob Σ ->
-  closed_env Σ ->
-  closedn 0 a ->
   Ee.eval Σ a a' -> isEtaExp Σ [] a -> isEtaExp Σ [] a'.
 Proof.
-  intros etaΣ wfΣ HΣcl Hcl.
+  intros etaΣ wfΣ.
   induction 1 using eval_mkApps_rect.
   all:try simp isEtaExp; rewrite -!isEtaExp_equation_1 => //.
-  - move/isEtaExp_tApp'.
+  6:{  
+    move/isEtaExp_tApp'.
     destruct decompose_app eqn:da.
     destruct expanded_head_viewc eqn:vc.
     * move => [hl [hf [ha /andP[] ise etal]]].
       rewrite hf in H. eapply eval_construct in H as [? []]. exfalso. solve_discr.
     * move => [hl [hf [ha /andP[] /andP[] etal etab]]] isel.
-      unfold isEtaExp_fixapp in etal. destruct nth_error eqn:Efix; try easy.
-      (* maybe the new relation does not preserve eta-expandedness? it's certainly hard to prove.
-
-         From H we can get that remove_last l was long enough to trigger evaluation, so the shorter application is still expanded
+      pose proof (mkApps_app (EAst.tFix mfix idx) argsv [av]).
+      cbn in H3. rewrite <- H3. clear H3.
+      subst.
+      eapply eval_mkApps_tFix_inv in H as [[(? & Heq) | (args' & n & ? & ? & ? & Heq)] | (? & ? & ? & ? & ?)]; eauto.
+      -- eapply (f_equal decompose_app) in Heq. rewrite !decompose_app_mkApps in Heq => //. invs Heq.
+         rewrite isEtaExp_mkApps => //.
+         assert (l = [a]) as ->. { destruct l; cbn in H; try congruence. rewrite Nat.sub_0_r in H. cbn in ha. destruct l; cbn in *; try congruence. }
+         cbn [expanded_head_viewc]. rtoProp. repeat split.
+         ++ unfold isEtaExp_fixapp in *. destruct nth_error eqn:Hn; try easy.
+         ++ solve_all.
+         ++ solve_all. cbn. repeat econstructor. eapply IHeval2. now invs isel.  
+       -- eapply (f_equal decompose_app) in Heq. rewrite !decompose_app_mkApps in Heq => //. invs Heq.
+         rewrite isEtaExp_mkApps => //.
+         cbn [expanded_head_viewc]. rtoProp. repeat split.
+         ++ unfold isEtaExp_fixapp in *. destruct nth_error eqn:Hn; try easy. len.
+            eapply Nat.ltb_lt in etal.
+            eapply Nat.ltb_lt. sq. eapply All2_length in H3.
+            rewrite skipn_length in H3. lia.
+            rewrite firstn_length. rewrite remove_last_length' in H3, H4 |-*. eauto. lia.
+         ++ solve_all.
+         ++ sq. solve_all. eapply All_app_inv. 2:{ repeat econstructor. eapply IHeval2. rewrite ha. eapply Forall_last; eauto. }
+            eapply All_app_inv. repeat eapply All_firstn; eauto.
+            todo "strengthen IH".
+       -- rewrite !isEtaExp_mkApps in IHeval1 |- * => //.
+          cbn [expanded_head_viewc] in *. forward IHeval1; rtoProp.
+          ++ repeat split; solve_all. 2:{ unfold remove_last. now eapply All_firstn. }
+             unfold isEtaExp_fixapp, cunfold_fix in *. destruct nth_error; invs H1.
+             destruct nth_error; invs H3. eapply Nat.ltb_lt in etal. eapply Nat.ltb_lt. len.
+             destruct l; try congruence. cbn. rewrite remove_last_length' in H4; try congruence. cbn in *. lia.
+          ++ repeat split; solve_all. 2:{ eapply All_app_inv; eauto. repeat econstructor; eauto. eapply IHeval2. rewrite ha. eapply Forall_last; eauto. }
+             unfold isEtaExp_fixapp, cunfold_fix in *. destruct nth_error; invs H1.
+             destruct nth_error; invs H3. eapply Nat.ltb_lt in H5, etal. eapply Nat.ltb_lt. len.
+             destruct l; try congruence. cbn. rewrite remove_last_length' in H4; try congruence. cbn in *. lia.
+      * intros (? & ? & ? & ?). rtoProp. solve_all.
+        rewrite nth_error_nil in H6. easy.
+      * move/and4P => [] etat etal etaf etaa.
+        pose proof (mkApps_app (tFix mfix idx) argsv [av]). cbn in H3. rewrite <- H3. clear H3.
+        specialize (IHeval1 etaf). 
+        rewrite !isEtaExp_mkApps in IHeval1 |- * => //.
+        cbn [expanded_head_viewc] in *. rtoProp. repeat split; solve_all.
+        -- unfold isEtaExp_fixapp, cunfold_fix in *. destruct nth_error; invs H1.
+           len. eapply Nat.ltb_lt. eapply Nat.ltb_lt in H3. lia.
+        -- eapply All_app_inv; solve_all.
+  }
+  5:{
+    move/isEtaExp_tApp'.
+    destruct decompose_app eqn:da.
+    destruct expanded_head_viewc eqn:vc.
+    * move => [hl [hf [ha /andP[] ise etal]]].
+      rewrite hf in H. eapply eval_construct in H as [? []]. exfalso. solve_discr.
+    * move => [hl [hf [ha /andP[] /andP[] etal etab]]] isel.
+      subst.
+      eapply IHeval3.
       
-      *)
-      rewrite hf in H. eapply IHeval3. admit.
-      eapply etaExp_csubst; eauto. admit.
-      eapply IHeval2. admit.
-      solve_all. admit.
-      simp_eta in IHeval1.
-      eapply IHeval1.
-      subst. cbn in Hcl. rtoProp. eauto.
-      subst. econstructor.
-    * todo "rel".
-    * move/and4P => [] etat etal etaf etaa.
-      move / andP : Hcl => [] Hcl1 Hcl2; fold closedn in *.
-      eapply IHeval3; eauto.
-      { eapply closed_csubst. eapply eval_closed; eauto. eapply eval_closed in H; eauto. }
-      move: (IHeval1 Hcl1 etaf); simp_eta => etab.      
-      eapply etaExp_csubst; eauto.
-      { eapply eval_closed; eauto. }
-  - admit.
-  - move : Hcl => /andP [] Hcl1 Hcl2; fold closedn in *.  
-    rtoProp; intuition eauto.
+      pose proof (mkApps_app fn argsv [av]).
+      cbn in H3. rewrite <- H3. clear H3.
+
+      assert (isEtaExp Σ [] a). { rewrite ha. eapply Forall_last; eauto. solve_all. }
+
+      eapply eval_mkApps_tFix_inv in H as [[(? & Heq) | (args' & n & ? & ? & ? & Heq)] | (? & ? & ? & ? & ?)]; eauto.
+      -- eapply (f_equal decompose_app) in Heq. rewrite !decompose_app_mkApps in Heq => //. invs Heq.
+         assert (l = [a]) as ->. { destruct l; cbn in H; try congruence. rewrite Nat.sub_0_r in H. cbn in ha. destruct l; cbn in *; try congruence. }
+         eapply isEtaExp_mkApps_intro.
+         eapply isEtaExp_cunfold_fix. 2: eauto. solve_all.
+         now rewrite app_nil_r in H5. repeat econstructor. eauto.
+       -- eapply (f_equal decompose_app) in Heq. rewrite !decompose_app_mkApps in Heq => //. invs Heq. sq.
+         eapply isEtaExp_mkApps_intro. 
+         eapply isEtaExp_cunfold_fix. 2: eauto. solve_all.
+         now rewrite app_nil_r in H7.
+         eapply All_app_inv. 2: repeat econstructor; eauto.
+         eapply All_app_inv. repeat eapply All_firstn. solve_all.
+         todo "strengthen IH".
+       -- forward IHeval1.
+          rewrite isEtaExp_mkApps => //.
+          cbn [expanded_head_viewc]. rtoProp. repeat split; solve_all.
+          2: eapply All_firstn; eauto.
+          unfold isEtaExp_fixapp, cunfold_fix in etal, H4 |- *.
+          destruct nth_error; try easy. invs H4. eapply Nat.ltb_lt. lia.
+          rewrite isEtaExp_mkApps in IHeval1 => //.
+          cbn [expanded_head_viewc] in IHeval1. rtoProp.
+          eapply isEtaExp_mkApps_intro. 
+          eapply isEtaExp_cunfold_fix. 2: eauto. solve_all.
+          now rewrite app_nil_r in H9.
+          eapply All_app_inv. 2: repeat econstructor; eauto.
+          solve_all.
+        * intros (? & ? & ? & ?). rtoProp. solve_all.
+          rewrite nth_error_nil in H6. easy.
+        * move/and4P => [] etat etal etaf etaa. eapply IHeval3.
+          pose proof (mkApps_app fn argsv [av]). cbn in H3. rewrite <- H3. clear H3.
+          specialize (IHeval1 etaf). 
+          rewrite !isEtaExp_mkApps in IHeval1 => //.
+          cbn [expanded_head_viewc] in *. rtoProp.
+          eapply isEtaExp_mkApps_intro. 
+          eapply isEtaExp_cunfold_fix. 2: eauto. solve_all.
+          now rewrite app_nil_r in H6.
+          eapply All_app_inv. 2: repeat econstructor; eauto.
+          solve_all.
+  }
+  10:{ move/isEtaExp_tApp'.
+  destruct decompose_app eqn:da.
+  destruct expanded_head_viewc.
+  * move=> [] hl [] hf [] ha /andP[] hl' etal.
+    move: H H0. rewrite hf => H H0.
+    destruct (eval_construct_size H) as [args' []]. subst f'.
+    rewrite -[EAst.tApp _ _](mkApps_app _ _ [a']).
+    rewrite isEtaExp_Constructor.
+    apply/andP; split => //.
+    + len. eapply All2_length in a0. rewrite -a0.
+      rewrite (remove_last_last l a) // in hl'.
+      rewrite app_length in hl'.
+      now cbn in hl'.
+    + solve_all.
+      rewrite (remove_last_last l a) // in etal.
+      eapply All_app in etal as [etal etaa].
+      depelim etaa. clear etaa. rewrite -ha in i.
+      eapply All_app_inv; try constructor; eauto.
+      clear -H0 a0 etal. solve_all.
+      destruct b as [ev Hev]. eapply (H0 _ _ ev) => //. lia.
+  * move => [hl [hf [ha /andP[] /andP[] etal etab]]] isel.
+    subst.
+  
+    assert (isEtaExp Σ [] a). { rewrite ha. eapply Forall_last; solve_all. }
+    assert (guarded : with_guarded_fix) by todo "guarded".
+    
+    destruct (eval_mkApps_tFix_inv _ _ _ _ _ guarded H) as [[(? & Heq) | (args' & n & ? & ? & ? & Heq)] | (? & ? & ? & ? & ?)]; eauto.
+    -- subst. cbn in H1. destruct with_guarded_fix; easy.
+    -- subst. rewrite guarded in H1. rewrite isFixApp_mkApps in H1 => //. destruct EAst.isLambda; easy.
+    -- eapply (isEtaExp_mkApps_intro _ _ f' [a']); eauto.
+       eapply IHeval1. rewrite isEtaExp_mkApps => //.
+      cbn [expanded_head_viewc]. rtoProp.
+      repeat split; solve_all.
+      2: eapply All_firstn; eauto.
+      unfold isEtaExp_fixapp,  cunfold_fix in *.
+      destruct nth_error; try easy.
+      invs H5. eapply Nat.ltb_lt. lia.
+  }
+  1:{ move/isEtaExp_tApp'.
+      destruct decompose_app eqn:da.
+      destruct expanded_head_viewc.
+      * move=> [] hl [] hf [] ha /andP[] hl' etal.
+        move: H H0. rewrite hf => H H0.
+        eapply eval_construct in H as [? []];solve_discr.
+      * solve_all. rtoProp. solve_all. subst.
+        eapply eval_mkApps_tFix_inv in H as [[(? & Heq) | (args' & n & ? & ? & ? & Heq)] | (? & ? & ? & ? & ?)]; eauto; try solve_discr; eauto. 3: todo "guarded".
+        -- invs Heq.
+        -- eapply IHeval3. eapply etaExp_csubst. eapply IHeval2.
+           rewrite H3. eapply Forall_last; solve_all.
+           forward IHeval1.
+           rewrite isEtaExp_mkApps => //.
+           cbn [expanded_head_viewc]. rtoProp; solve_all; solve_all.
+           2: eapply All_firstn; solve_all.
+           unfold isEtaExp_fixapp, cunfold_fix in *.
+           destruct nth_error; try easy. invs H4. eapply Nat.ltb_lt. lia.
+           simp_eta in IHeval1. eauto.
+       * solve_all. rtoProp. solve_all. rewrite nth_error_nil in H5; easy.
+  * move/and4P => [] etat etal etaf etaa. simp_eta in IHeval1. eapply IHeval3, etaExp_csubst; eauto.  
+  }
+
+  - rtoProp. solve_all. eapply IHeval2, etaExp_csubst; eauto. 
+
+  - rtoProp; intuition eauto.
     eapply IHeval2. rewrite /iota_red.
-    { eapply closed_substl.
-       eapply eval_closed in H; eauto. rewrite closedn_mkApps in H. rtoProp. solve_all. eapply All_skipn. solve_all.
-      solve_all. eapply All_nth_error in H6 as []; eauto. revert i. len. now rewrite H2.
-    }
     eapply isEtaExp_substl with (Γ := repeat 0 #|br.1|); eauto.
-    { len. rewrite List.skipn_length repeat_length in H2 |- *. lia. }
-    { eapply eval_closed in H; eauto. rewrite closedn_mkApps in H. rtoProp. solve_all. eapply All_skipn. solve_all. }
-    rewrite isEtaExp_Constructor // in H7. solve_all.
-    eapply All_skipn. move/andP: H7 => []. repeat solve_all.
+    { len. lia. }
+    rewrite isEtaExp_Constructor // in H4. solve_all.
+    eapply All_skipn. move/andP: H4 => []. repeat solve_all.
     eapply forallb_nth_error in H6; tea.
     now erewrite H1 in H6.
   - rtoProp; intuition auto.
-    eapply IHeval2. eapply isEtaExp_substl.
+    eapply IHeval2. eapply isEtaExp_substl. shelve.
     now apply forallb_repeat.
     rewrite H2 in H6. simpl in H6.
     now move/andP: H6.
-  - intros ise.
-    eapply IHeval3.
-    apply isEtaExp_tApp' in ise.
-    destruct decompose_app eqn:da.
-    destruct (cc_viewc t) eqn:cv.
-    * destruct ise as [? [? []]]. rewrite H4 in H.
-      eapply eval_construct in H as [? []];solve_discr.
-    * todo "fix". 
-    * move/and4P: ise => [] iset isel isef isea.
-      rewrite -[EAst.tApp _ _](mkApps_app _ _ [av]).
-      specialize (IHeval1 isef).
-      rewrite isEtaExp_mkApps // in IHeval1.
-      simp cc_viewc in IHeval1.
-      move: IHeval1 => /andP [] / andP [] evrarg evfix evargs.
-      eapply isEtaExp_mkApps_intro.
-      eapply isEtaExp_cunfold_fix; tea.
-      simp isEtaExp in evfix.
-      eapply All_app_inv. now solve_all. constructor; auto.
-  - intros ise.
-    apply isEtaExp_tApp' in ise.
-    destruct decompose_app eqn:da.
-    destruct (cc_viewc t) eqn:cv.
-    * destruct ise as [? [? []]]. rewrite H4 in H.
-      eapply eval_construct in H as [? []]; solve_discr.
-    * todo "fix".
-    * move/and4P: ise => [] iset isel isef isea.
-      rewrite -[EAst.tApp _ _](mkApps_app _ _ [av]).
-      specialize (IHeval1 isef).
-      rewrite isEtaExp_mkApps // in IHeval1.
-      simp construct_viewc in IHeval1.
-      move: IHeval1 => /andP [] / andP [] evrarg evfix evargs.
-      todo "fix". (* 
-      eapply isEtaExp_mkApps_intro => //.
-      eapply All_app_inv. now solve_all. constructor; auto. *)
+    Unshelve. now len.
+  - todo "unguarded".
   - move=> /andP[] hdiscr hbrs. specialize (IHeval1 hdiscr).
     move: IHeval1. rewrite isEtaExp_mkApps // /= => /andP[] hcof hargs.
     eapply IHeval2. simp_eta. rtoProp; intuition auto.
     apply isEtaExp_mkApps_intro; solve_all.
     eapply (isEtaExp_cunfold_cofix _ mfix idx); tea.
-    simp_eta in hcof.
-  -  move=> hdiscr. specialize (IHeval1 hdiscr).
+    simp_eta in hcof. solve_all. now rewrite app_nil_r in H2.
+  - move=> hdiscr. specialize (IHeval1 hdiscr).
     move: IHeval1. rewrite isEtaExp_mkApps // /= => /andP[] hcof hargs.
     eapply IHeval2. simp_eta.
     apply isEtaExp_mkApps_intro; solve_all.
     eapply (isEtaExp_cunfold_cofix _ mfix idx); tea.
-    simp_eta in hcof.
+    simp_eta in hcof. solve_all. now rewrite app_nil_r in H2.
   - move=> _. eapply IHeval. eapply isEtaExp_lookup in H; tea.
     now move: H; rewrite /isEtaExp_decl /= /isEtaExp_constant_decl H0 /=.
   - intros hd.
@@ -1256,30 +1448,9 @@ Proof.
     destruct nth_error eqn:hnth.
     rewrite isEtaExp_Constructor.
     destruct args => //. now rewrite nth_error_nil in hnth.
-    move=> /andP[] _ hargs. eapply nth_error_forallb in hnth; tea.
+    move=> /andP[] _ hargs.
+    eapply nth_error_forallb in hnth; tea.
     depelim H0. now cbn in H1.
-  - move/isEtaExp_tApp'.
-    destruct decompose_app eqn:da.
-    destruct cc_viewc.
-    * move=> [] hl [] hf [] ha /andP[] hl' etal.
-      move: H H0. rewrite hf => H H0.
-      destruct (eval_construct_size H) as [args' []]. subst f'.
-      rewrite -[EAst.tApp _ _](mkApps_app _ _ [a']).
-      rewrite isEtaExp_Constructor.
-      apply/andP; split => //.
-      + len. eapply All2_length in a0. rewrite -a0.
-        rewrite (remove_last_last l a) // in hl'. len in hl'.
-        now cbn in hl'.
-      + solve_all.
-        rewrite (remove_last_last l a) // in etal.
-        eapply All_app in etal as [etal etaa].
-        depelim etaa. clear etaa. rewrite -ha in i.
-        eapply All_app_inv; try constructor; eauto.
-        clear -H0 a0 etal. solve_all.
-        destruct b as [ev Hev]. eapply (H0 _ _ ev) => //. lia.
-    * todo "fix".
-    * move/and4P => [] etat etal etaf etaa.
-      eapply (isEtaExp_mkApps_intro _ f' [a']); eauto.
 Qed.
 
 Lemma isEtaExp_eval Σ {wfl : WcbvFlags} t v  :
